books/evm/env-defthms.lisp
@@ -2,11 +2,49 @@
 
 (include-book "context-defthms")
 (include-book "env")
+(include-book "memory-defthms")
 (include-book "stack-defthms")
 (include-book "substate-defthms")
 
 (defthm mk-env-op-validp
     (env/validp (mk-env-op anything)))
+
+(defthm env/set-pc-validp
+    (implies (env/validp e)
+             (env/validp (env/set-pc e n))))
+
+(defthm env/stack/popn-validp
+    (implies (env/validp e)
+             (env/validp (env/stack/popn e n))))
+
+(defthm env/stack/push-validp
+    (implies (env/validp e)
+             (env/validp (env/stack/push e v))))
+
+(defthm env/memory/store-byte-validp
+    (implies (env/validp e)
+             (env/validp (env/mem/store-byte e addr v)))
+  :hints (("Goal"
+           :in-theory (e/d () (memory/validp memory/store-byte))
+           :use ((:instance memory-store-byte-validp
+                            (m (nth 2 (cdr e))))))))
+
+(defthm env/memory/store-byte-array-validp
+    (implies (env/validp e)
+             (env/validp (env/mem/store-byte-array e addr v))))
+
+(defthm env/memory/store-w256-validp
+    (implies (env/validp e)
+             (env/validp (env/mem/store-w256 e addr v))))
+
+(defthm env/storage/store-validp
+    (implies (env/validp e)
+             (env/validp (env/storage/store e offset v))))
+
+(defthm env/set-halted-validp
+    (implies (and (env/validp e)
+                  (halted/validp h))
+             (env/validp (env/set-halted e h))))
 
 (defthm env/setsubstate-io-validp
     (implies (and (env/validp e)
