books/evm/op-exec-defthms.lisp
@@ -6,6 +6,20 @@
 (include-book "env-defthms")
 (include-book "op-exec")
 
+(defthm op-unchanged-in-exec-swap-swapper
+    (equal (car (exec-swap-swapper e n))
+           (car e)))
+
+(defthm exec-swap-swapper-validp
+    (implies (env/validp e)
+             (env/validp (exec-swap-swapper e n))))
+
+(defthm exec-swap-helper-validp
+    (implies (env/validp e)
+             (env/validp (exec-swap-helper e n)))
+  :hints (("Goal"
+           :in-theory (e/d () (env/validp exec-swap-swapper env/pc+n)))))
+
 (defthm exec-stop-io-validp
     (implies (env/validp e)
              (env/validp (exec-stop e))))
